\documentclass[9pt]{memoir}

\usepackage[margin=1cm]{geometry}
\usepackage{multicol}
\usepackage{amsmath, amsfonts, amssymb, mathtools}
\usepackage{graphicx}
\usepackage{ulem}
\usepackage{macros-common}
\usepackage{xcolor}

\makepagestyle{myplain}
\makeevenhead{myplain}{\footnotesize \thepage}{}{\footnotesize MAS365 Cheatsheet}
\makeoddhead{myplain}{\footnotesize MAS365 Cheatsheet}{}{\footnotesize \thepage}

\makeevenfoot{myplain}{}{}{}
\makeoddfoot{myplain}{}{}{}

\pagestyle{myplain}

\makeatletter
\newcommand{\ostar}{\mathbin{\mathpalette\make@circled\star}}
\newcommand{\make@circled}[2]{%
  \ooalign{$\m@th#1\smallbigcirc{#1}$\cr\hidewidth$\m@th#1#2$\hidewidth\cr}%
}
\newcommand{\smallbigcirc}[1]{%
  \vcenter{\hbox{\scalebox{0.77778}{$\m@th#1\bigcirc$}}}%
}
\makeatother

\begin{document}

\setlength\columnsep{20pt}
\begin{multicols*}{3}
    \parindent=0pt
    \abovedisplayskip=3pt
    \belowdisplayskip=3pt
    \parskip=5pt
    \allowdisplaybreaks
    \def\nl{\hspace*{\fill}\\}
    \def\s{$\mathllap{\bullet\ \>}$}

    \setcounter{chapter}{1}
    \section{Arith Using Computer}

    \s \textbf{IEEE double} 64-bit floating \#
    $$\uline{sc_{10}\cdots c_0 f_{-1}\cdots f_{-52}} = (-1)^s 2^{c-1023}(1+f),$$
    $c=(c_{10}\cdots c_0)_2$ and $f=(0.f_{-1}\cdots f_{-52})_2$.

    \s \textbf{Underflow} $<2^{-1022}(1+0)$, \nl
    \s \textbf{Overflow} $>2^{1023}(2-2^{-52})$,

    \s \textbf{Actual error} $p_{true}-p_{app}$, \nl
    \s \textbf{Absolute error} $|p_{true}-p_{app}|$, \nl
    \s \textbf{Relative error} $|p_{true}-p_{app}|/|p_{true}|$, \nl
    \s $p^*$ approx. $p$ to $\boldsymbol t$ \textbf{significant digits} if
    $$ \frac{\abs{p-p^*}}{|p| }\le 5\times 10^{-t} $$

    \s $k$-digit chop: $\text{rel err}\le 10^{-k+1}$, \nl
    \s $k$-digit round: $\text{rel err}\le 10^{-k+1}$

    \s \textbf{Finite digit arith} $x\ostar y = fl(fl(x)\star fl(y))$

    \s \textbf{Err growth} $\epsilon_n = O(n)\epsilon_0$ linear; \nl
    \hspace*{0.5cm}$\epsilon_n = O(C^n)\epsilon_0$ ($C>1$) exponential

    \s $|\alpha_n-\alpha| = O(\beta_n)\implies \alpha_n\to\alpha$ with \textbf{rate of conv} $O(\beta_n)$

    \setcounter{chapter}{2}
    \setcounter{section}{0}
    \section{Err Analysis}
    \s {Order of convergence}: $p_n \to p$ \textbf{of order $\boldsymbol \alpha$ with asympt err const $\boldsymbol\lambda$} if ($\alpha,\lambda>0$)
    $$ \frac{\abs{p_{n+1}-p}}{\abs{p_n-p}^\alpha} \to \lambda $$
    \s $\alpha=1$, $\lambda=1$: sublinearly conv,\nl
    $\alpha=1$, $\lambda\in(0,1)$: linearly conv,\nl
    $\alpha=1$, $\lambda=0$: superlinearly conv,\nl
    $\alpha=2$: quad'ly conv\nl
    \s $g\in C[a,b]$, $g\in C^1(a,b)$, $|g'(x)|\le {^\exists k}<1$ on $(a,b)$, $g(p)=p$, $g'(p)\ne 0$, $p_0\ne p\in [a,b]$\nl  then $p_n=g(p_{n-1})\to p$ linearly. \nl
    \s $g\in C^2$, $g(p)=p$, $g'(p)=0$, $|g''(x)|<M$, \nl
    then $\exists\delta>0$ so that $p_0\in [p-\delta,p+\delta]$ implies $p_n=g(p_{n-1})\to p$ at least quad'ly with
    $$ \abs{p_{n+1}-p} < \frac M2 \abs{p_n-p}^2. $$

    \section{Bisection Method}
    \s Stopping crit: $|p_n - p_{n-1}|/|p_n| < \epsilon$, $p_n\ne 0$ \nl
    \s Abs err: $|p_n - p| \le (b-a)\,2^{-n}$. \nl
    \s $a_n + (b_n-a_n)/2$ is computationally better than $(a_n+b_n)/2$ when $b_n-a_n$ is near the max precision \nl
    \s $\sgn f(a)\cdot \sgn f(b)<0$ is better than $f(a)f(b)<0$ due to over/underflow

    \section{Fixed Point Iteration}
    \s $g\in C[a,b],[a,b]\to [a,b]\implies \exists$ a fixed pt\nl
    \s $g'(x)<{^\exists k} < 1$ on $(a,b)\implies \exists!$ f.p.,\nl
    \hspace*{\fill}$|p_n| \le k^n \max\set{p_0-a,b-p_0}$,\\
    \hspace*{\fill}$|p_n| \le k^n\abs{p_1-p_0}/(1-k)$.

    \section{Newton's Method}
    \s $p_n = p_{n-1} - {f(p_{n-1})}/{f'(p_{n-1})}.$ \nl
    If $f\in C^2[a,b]$, $p\in(a,b)$, $f(p)=0$, $f'(0)\ne 0$, then $\exists \delta>0$ s.t. $|p_0-p|\le \delta\implies p_n\to p$ quadratically. \nl[1mm]
    \s \textbf{Secant method}
    $$ p_n = p_{n-1} - f(p_{n-1}) {\Big/} \frac{f(p_{n-1})-f(p_{n-2})}{p_{n-1}-p_{n-2}}$$
    \s \textbf{Method of false position}
    $p_0,p_1$ w/ $f(p_0)f(p_1)<0$,
    $$ p_2 = p_1 - \frac{f(p_1)(p_1-p_0)}{f(p_1)-f(p_0)},$$
    If $f(p_{n-1})\cdot f(p_{n-2})\ge 0$, redefine $p_{n-2}\leftarrow p_{n-3}$. Calculate:
    $$ p_n = p_{n-1} - \frac{f(p_{n-1})(p_{n-1}-p_{n-2})}{f(p_{n-1}) - f(p_{n-2})}. $$
    \s \textbf{Modified Newton}
    When $p$ is of multiplicity $m$, replace $f$ by $\mu(x) =f(x)/f'(x)$ and do the same proc
    $$ p_n = p_{n-1} - \mu(p_{n-1})/\mu'(p_{n-1})$$

    \section{Aitken's $\boldsymbol{\Delta^2}$ Method}
    \s If $p_n\to p$ linearly, then
    $$ \hat p_n = p_n - \frac{(p_{n+1}-p_n)^2}{p_{n+2}-2p_{n+1}+p_n} \to p $$
    sublinearly.  \nl
    \s \textbf{Steffensen's} For a problem finding $g(p)=p$, define $\hat p_{-1} = p_0$, $\hat p_n = \set{\Delta^2} (\hat p_{n-1})$ where
    $$ \set{\Delta^2}(x) = x - \frac{ (g(x) - x)^2 }{ g(g(x)) - 2g(x) + x }. $$
    It is the same with finding a root of $f(x) \coloneqq g(x) - x$ with the following iterator:
    $$ s(x) = x - \frac{f(x)}{(f(x+h)-f(x))/h},\quad h=f(x) $$

    \section{Horner's Method}
    \s $P(x)=a_n x^n+\cdots + a_0$, $b_n = a_n$ and $b_k = a_k + b_{k+1}x_0$ for $k=n-1,\dots,0$. Then $b_0=P(x_0)$ and
    $$ Q(x)=b_nx^{n-1}+\cdots + b_2x + b_1 $$
    satisfies $P(x) = (x-x_0)Q(x) + b_0$ and $P'(x_0)=Q(x_0)$.

    \s One can repeat this to get an approximate factorization of $P$.

    \section{M\"uller's Method}
    For $(p_i,f(p_i))$ ($i=0,1,2$), determine $p_3$ by a root (closer to $p_2$) of the quadratic polynomial $P$ agreeing at the given point.
    $$ f(p_i) = a(p_i - p_2)^2 + b(p_i - p_2) + c, $$
    $$ p_3 - p_2 = \frac{-2c}{b \pm \sqrt{b^2-4ac}}. $$

    \setcounter{chapter}{3}
    \setcounter{section}{0}
    \section{Lagrange Interpolation}
    \s $(n+1)$-point interpolation:
    $$P(x) = \sum_{k=0}^n f(x_k) L_{n,k}(x)$$
    where
    $$ L_{n,k}(x) = \prod_{j\ne k}\frac{x-x_j}{x_k-x_j}$$
    with
    $$ f(x) = P(x) + \frac{f^{(n+1)}(\xi)}{(n+1)!}(x-x_0)\cdots (x-x_n) $$
    for some $\xi \in \text{int\,ConvHull}\set{x_0,\cdots ,x_n}$.
    \s \textbf{Generalized Rolle's theorem} $f\in C[a,b]$, $n$ times diff'ble on $(a,b)$. If $f(x)=0$ at $a\le x_0<\dots<x_n\le b$, then $\exists c \in (a,b)$, $f^{(n)}(c)=0$. \nl
    \s Runge phenomenon: a problem of oscillation at the edges of an interval that occurs when using polynomial interpolation with polynomials of high degree over a set of equispaced interpolation points.

    \section{Neville's Method}
    \s Letting $P_{S}(x)$ be the Lagrange interp'n poly agreeing at $x_s\ (s\in S)$, then $ P_{[k]}(x) $ equals to the following: ($[k] = \{0,\dots,k\}$)
    $$\frac{(x-x_j)P_{[k]-\{j\}}(x) - (x-x_i) P_{[k]-\set{i}}(x)  }{ x_i-x_j } $$
    \s With $Q_{i,j} = P_{i-j,i-j+1,\dots,i}$ $(i\ge j)$, $f(x_i) = Q_{i,0}$ and
    $$ Q_{i,j} = \frac{(x-x_{i-j}) Q_{i,j-1} - (x-x_i)Q_{i-1,j-1} }{x_i-x_{i-j}} $$

    \section{Divided Differences}
    $$f[x_{a,\cdots,b}] = \frac{f[x_{a+1,\dots,b}] - f[x_{a,\dots,b-1}]}{x_b-x_a}$$

    For $x=x_0+sh = x_n + s'h$ $(h=x_i-x_{i-1})$,
    \begin{align*}
        P_n(x) & = \sum_{k=0}^n f[x_0,\dots,x_k]\prod_{j=0}^{k-1}(x-x_j)
        \\&= \sum_{k=0}^n \binom s k \Delta^k f(x_0)
        \\&= \sum_{k=0}^n f[x_n,\dots,x_{n-k}]\prod_{j=n}^{n-k+1}(x-x_j)
        \\&= \sum_{k=0}^n (-1)^k \binom {-s'} k \nabla^k f(x_n)
    \end{align*}
    When $n=2m+1$ is odd, with pts $x_{-m-1, \dots, 0,\dots,m+1}$ and $x=x_0+sh$, (Stirling's formula)
    \begin{align*}
        P_n(x) & = f[x_0] + \frac{sh}2 (f[x_{-1},x_0]+f[x_0,x_1])
        \\&\quad + s^2h^2 f[x_{-1},x_0,x_1]
        \\ &\mkern-30mu +\frac{s(s^2-1^2)h^3}{2} (f[x_{-2,-1,0,1}]+f[x_{-1,0,1,2}])
        \\ &+\cdots
        \\ &+ s^2(s^2-1^2)\cdots(s^2-(m-1)^2)h^{2m} \cdot
        \\ & \mkern160mu f[x_{-m},\cdots,x_m]
        \\ &+ \frac{s(s^2-1^2)\cdots (s^2-m^2)h^{2m+1}} 2 \cdot
        \\ &  \mkern-20mu (f[x_{-m},\cdots,x_{m+1}]+f[x_{-m-1},\cdots,x_m])
    \end{align*}
    where the last term disappears when $n=2m$ (with points $x_{-m,\dots,m}$).

    \section{Hermite Polynomials}
    $f\in C^1[a,b]$, $x_0,\dots,x_n\in [a,b]$ distinct, the unique poly of least degree agreeing w/ $f$ and $f'$ at $x_0,\dots,x_n$ is
    $$H_{2n+1} = \sum_{j=0}^n f(x_j)H_{n,j} + \sum_{j=0}^n f'(x_j)\hat H_{n,j}$$
    where $H_{n,j} = [1-(x-x_j)L'_{n,j}(x_j)]L_{n,j}^2(x)$ and $\hat H_{n,j}(x) = (x-x_j)L^2_{n,j}(x)$, with the error
    \begin{align*}
        f(x) & = H_{2n+1}(x)
        \\ &+ \frac{(x-x_0)^2\cdots(x-x_n)^2}{(2n+2)!}f^{(2n+2)}(\xi),
    \end{align*}
    $\xi\in(a,b)$. \nl
    \s Divided differences: with points $x_0,x_0,$ $x_1,x_1,$ $\dots,x_k,x_k$, use the div diff formula with $f[x_j]\coloneqq f(x_j)$, $f[x_j,x_j] \coloneqq f'(x_j)$.

    \section{Cubic Splines}
    \s $x_0,x_1,\dots,x_n$ \nl
    \s $S(x) = S_j(x)$ on $[x_j,x_{j+1}]$, $S_j$ cubic with
    $$ S_j(x_j)=f(x_j),\ S_j(x_{j+1})=f(x_{j+1})  $$
    for $j=0,\dots,n-1$,
    $$ S_{j+1}'(x_{j+1})=S_j'(x_{j+1}),$$ $$S_{j+1}''(x_{j+1})=S_j''(x_{j+1}) $$
    for $j=0,\dots,n-2$, and with one of the following: \nl
    \s (natural bd)\quad $ S''(x_0)=S''(x_n)=0, $ \nl
    \s (clamped bd) $$S'(x_0)=f'(x_0),\quad S'(x_n)=f'(x_n).$$

    \s Construction (natural cubic spl):
    \begin{align*}
        S_j(x)     & = a_j+\cdots+ d_j(x-x_j)^3, \\
        a_j        & = f(x_j),\quad h_j = x_{j+1} - x_j, \\
        A\mathbf x & = \mathbf b\quad \text{where}
    \end{align*}
    \begin{align*}
        A         & = \begin{pmatrix}
            1      & 0                      & 0                                 & \cdots  & \cdots             & 0       \\
            h_0    & 2(h_0+h_1) \mkern-15mu & h_1                               & \ddots  &                    & \vdots  \\
            0      & h_1                    & \mkern-15mu 2(h_1+h_2)\mkern-15mu & h_2     & \ddots             & \vdots  \\
            \vdots & \ddots                 & \ddots                            & \ddots  & \ddots             & 0       \\
            \vdots &                        & \ddots                            & h_{n-2} & 2(h_{n-2}+h_{n-1}) & h_{n-1} \\
            0      & \cdots                 & \cdots                            & 0       & 0                  & 1       \\
        \end{pmatrix},                 \\
        \mathbf b & = \begin{pmatrix}
            0 \\ \frac 3{h_1}(a_2-a_1)-\frac 3{h_0}(a_1-a_0) \\ \vdots \\ \frac {3(a_n-a_{n-1})}{h_{n-1}}-\frac {3(a_{n-1}-a_{n-2})}{h_{n-2}} \\ 0
        \end{pmatrix},                 \\
        \mathbf x & = [c_0,\dots,c_n]^T,                         \\
        b_j       & = (a_{j+1} - a_j)/h_j - h_j(c_{j+1}+2c_j)/3, \\
        d_j       & = (c_{j+1}-c_j) / (3h_j).
    \end{align*}

    \s Construction (clamped cubic spl):
    \begin{align*}
        A         & = \begin{pmatrix}
            2h_0   & h_0                    & 0                                 & \cdots  & \cdots             & 0        \\
            h_0    & 2(h_0+h_1) \mkern-15mu & h_1                               & \ddots  &                    & \vdots   \\
            0      & h_1                    & \mkern-15mu 2(h_1+h_2)\mkern-15mu & h_2     & \ddots             & \vdots   \\
            \vdots & \ddots                 & \ddots                            & \ddots  & \ddots             & 0        \\
            \vdots &                        & \ddots                            & h_{n-2} & 2(h_{n-2}+h_{n-1}) & h_{n-1}  \\
            0      & \cdots                 & \cdots                            & 0       & h_{n-1}            & 2h_{n-1} \\
        \end{pmatrix}, \\
        \mathbf b & = \begin{pmatrix}
            \frac 3{h_0}(a_1-a_0)-3f'(a) \\ \frac 3{h_1}(a_2-a_1)-\frac 3{h_0}(a_1-a_0) \\ \vdots \\ \frac {3(a_n-a_{n-1})}{h_{n-1}}-\frac {3(a_{n-1}-a_{n-2})}{h_{n-2}} \\ 3f'(b) - \frac 3{h_{n-1}}(a_n-a_{n-1})
        \end{pmatrix},
    \end{align*}
    \s Error bound for clamped cub spl: \nl
    $f \in C^4[a,b]$ with $\max_{[a,b]}|f^{(4)}(x)| = M$. Then for the clampled cub spl interpolant to $f$ w.r.t. $a=x_0<\dots <x_n=b$,
    $$ |f(x)-s(x)| \le \frac{5M}{384}\max_{0\le j\le n-1} h_j^4 $$

    \s Not-a-knot condition: $S'''(x)$ is continuous at $x_1$ and $x_{n-1}$.\nl
    \s \textbf{Piecewise Cubic Hermite Polynomial}: Guide points
    $(x_0,y_0)$, $(x_0+\alpha_0,y_0+\beta_0)$, \uline{$(x_1-\alpha_1,y_1-\beta_1)$}, $(x_1,y_1)$. (Be careful for the signs) \nl
    $x(i)=x_i$, $x'(i)=\alpha_i$
    \begin{align*}
        x(t) & = [2(x_0-x_1)+(\alpha_0+\alpha_1)]t^3
        \\&+ [3(x_1-x_0)-(\alpha_1+2\alpha_0)]t^2
        \\&+\alpha_0 t + x_0,
    \end{align*}
    similarly for $y$ and $\beta$.

    \setcounter{chapter}{4}
    \setcounter{section}{0}
    \section{Numerical Differentiation}
    \s $(n+1)$-point formula: $x_0,\dots,x_n \in [a,b]$, $f\in C^{n+1}[a,b]$. Then $\exists\eta_1,\dots,\eta_n,\xi(x) \in (a,b)$ s.t.
    \begin{align*}
        f'(x) & = \sum_{k=0}^n f(x_k)L_{n,k}'(x)\\
        &+\frac{f^{(n+1)}(\xi)}{n!}(x-\eta_1)\cdots (x-\eta_n)
    \end{align*}
    (where $\eta_i \in (x_{i-1},x_i)$ at which $f'(\eta_i)=P'(\eta_i)$ by Rolle) \nl
    \\[3.2cm]
    Proof: using
    $$ g(t) = f'(t) - P'(t) - (f'(x) - P'(x))\prod \frac{t-\eta_j}{x-\eta_j} $$

    \s Three-pt midpt formula
    \begin{align*}
        \mkern-30mu f'(x_0) = \frac 1{2h} [f(x_0+h)-f(x_0-h)] - \frac{h^2}6 f^{(3)}(\xi)
    \end{align*}

    \s Three-pt endpt formula
    \begin{align*}
        f'(x_0) = \frac 1{2h} \Big[ & -3f(x_0)+4f(x_0+h)
        \\&\qquad -f(x_0+2h)\Big]+ \frac{h^2}3 f^{(3)} (\xi)
    \end{align*} \vskip3cm
    \s Five-pt midpt formula
    \begin{align*}
       & f'(x_0) = \frac 1{12h}\Big [f(x_0-2h)-8f(x_0-h)
        \\& +8f(x_0+h)-f(x_0+2h)\Big]+ \frac{h^4}{30} f^{(5)}(\xi)
    \end{align*}
    \s Five-pt endpt formula
    \begin{align*}
        f'(x_0) & = \frac 1{12h} \Big[-25f(x_0)+48f(x_0+h)
        \\&-36f(x_0+2h)+16f(x_0+3h)
        \\& -3f(x_0+4h)\Big]+\frac{h^4}{5} f^{(5)}(\xi)
    \end{align*}
    \s Second derivative midpt formula
    \begin{align*}
        f''(x_0) & = \frac 1{h^2}\Big [f(x_0-h)-2f(x_0)
        \\ &+f(x_0+h)\Big]-\frac{h^2}{12}f^{(4)}(\xi)
    \end{align*}
    \s Round-off err instability: with the round-off err bound $|e(x_0\pm h)|\le \varepsilon$ and $|f^{(3)}|\le M$, then the round-off err bound for the 3-pt midpt formula is $(e = f - \tilde f)$
    \begin{align*}
        \mkern-30mu\abs{f'(x_0) - \frac{\tilde f(x_0+h)-\tilde f(x_0-h)}{2h}}\le \frac\varepsilon h + \frac{h^2}6M
    \end{align*}
    minimized at $h=\sqrt[3]{3\varepsilon/M}$.

    \section{Richardson's Extrap}
    \s $O(h^j)$ extrapolation $N_j$:
    $$ N_j(h) = N_{j-1}\paren{h \over 2} + \frac{N_{j-1}(h/2)-N_{j-1}(h)}{2^{j-1}-1} $$
    \s For even $O(h^{2j})$ extrapolation $N_j$, replace $2^{j-1}-1$ by $4^{j-1}-1$.

    \section{Newton--Cotes}
    \s $(n+1)$-pt closed Newton--Cotes: $x_0=a,x_n=b,h=(b-a)/n$, error term is
    \begin{align*}
        \frac{h^{n+3}f^{(n+2)}(\xi)}{(n+2)!}\int_0^n t^2(t-1)\cdots (t-n)dt
    \end{align*}
    for even $n$ and $f\in C^{n+2}[a,b]$; and
    \begin{align*}
        \frac{h^{n+2}f^{(n+1)}(\xi)}{(n+1)!}\int_0^n t(t-1)\cdots (t-n)dt
    \end{align*}
    for odd $n$ and $f\in C^{n+1}[a,b]$.\nl
    \s Coeff for $n=1,2,3,4$: $\frac 12(1,1); \frac13(1,4,1); $\nl
    $\frac38(1,3,3,1); \frac{2}{45}(7,32,12,32,7).$ (Trapezoid, Simpson, Simpson $\frac 38$, Boole)\nl
    \s $(n+1)$-pt open Newton--Cotes: $x_{-1}=a,x_{n+1}=b,h=(b-a)/(n+2)$; \nl for the error term, replace $\int_0^n$ by $\int_{-1}^{n+1}$ in the above. \nl
    \s Coeff for $n=0,1,2,3$: $(2); \frac32(1,1); $\nl
    $\frac43 (2,-1,2); \frac 5{24}(11,1,1,11)$. ($n=0$: \uline{midpt rule}) \nl
    \s Compo Simpson err term: $-\frac{b-a}{180}h^4 f^{(4)}(\mu)$
    \s Compo Trapez err term: $-\frac{b-a}{12}h^2 f''(\mu)$
    \s Compo midpt rule: $h=(b-a)/(n+2)$, $n$ even,
    $$ \int_a^b f = 2h\sum_{\text{even }j}f(x_j) -\frac{b-a}{6}h^2 f''(\mu)$$
    \section{Gaussian Quadrature}
    $x_j$: roots of $n$-th Legendre poly,
    $$ c_i=\int_{-1}^1 \prod_{j\ne i}\frac{x-x_j}{x_i-x_j}\,dx,$$
$$ \int_{-1}^1 P(x)dx = \sum c_j P(x_j)$$
\end{multicols*}

\end{document}
